CellularAutomatas/proofs/is_two_stage_of_rt_closed_and_prefix_stable.lean
@@ -16,21 +16,11 @@ import CellularAutomatas.defs
 import CellularAutomatas.proofs.composition
 import CellularAutomatas.proofs.basic
 import CellularAutomatas.proofs.finite_state_transducers
+import CellularAutomatas.proofs.advice_prefix_mem_rt_closed
+import CellularAutomatas.proofs.two_stage_is_rt_closed
 
 namespace CellularAutomatas
 
-
-@[simp]
-lemma adv_empty (adv : Advice α Γ) : adv.f [] = [] := by
-  have h_len : (adv.f []).length = 0 := by simp [adv.len]
-  rw [List.length_eq_zero_iff.mp h_len]
-
-
-lemma tCellAutomatonWithAdvice.elem_L_iff {O: tCellAutomatonWithAdvice α}:
-  w ∈ O.L ↔ (O.adv.annotate w) ∈ O.C.L := by rfl
-
-
--- Reconstruct a two stage advice from a rt-closed and prefix-stable advice
 
 open Classical
 
@@ -38,119 +28,59 @@ open Classical
 variable {α: Type} [Alphabet α]
 variable {Γ: Type} [Alphabet Γ]
 
+
+lemma tCellAutomatonWithAdvice.elem_L_iff {α} {C: tCellAutomaton (α × Γ)} {adv: Advice α Γ} (w: Word α):
+    w ∈ (C + adv).L ↔ adv.annotate w ∈ C.L := by rfl
+
+
 def L_c (adv: Advice α Γ) (c: Γ) : Language α :=
   { w | (adv.f w).getLast? = some c }
 
 
-
-/-
-
-
+def CA_adv_L_c (α) [Alphabet α] (c : Γ) : CA_rt (α × Γ) :=
+  fix_empty false (toRtCa ((ca_id_word (α × Γ)).map_project (fun (_, g) => g == c)))
 
 
-
-* L_c := { w | adv.f(w).getLast? = c }
-* (prefix_mem L_c) is two_stage, because L_c is in L(RT-CA) by rt-closedness of adv
- h: adv.rt_closed
-* ((⊗ fun c => prefix_mem_two_stage L_c h).map_project first_true_or_default).advice = adv
--/
-
---
-
-namespace LcInRt
-
-
-def AdvCALc (c : Γ) : tCellAutomaton (α × Γ) := {
-  toCellAutomaton := (ca_id_word (α × Γ)).map_project (fun (_, g) => g == c)
-  t := fun n => n - 1
-  p := fun _ => 0
-}
-
-lemma myCA_in_rt (c : Γ) : AdvCALc c ∈ CA_rt (α × Γ) := by
-  simp [CA_rt, t_rt, AdvCALc, tCellAutomata, CA]
-
-
-
-def O (adv : Advice α Γ) (c : Γ) : tCellAutomatonWithAdvice α := ⟨Γ, adv, AdvCALc c⟩
-
-
-lemma O_L_eq_L_c (adv : Advice α Γ) (c : Γ) : (O adv c).L = L_c adv c := by
+lemma CA_adv_L_c_spec (adv : Advice α Γ) (c : Γ) : ((CA_adv_L_c α c).val + adv).L = L_c adv c := by
   ext w
-  simp [tCellAutomatonWithAdvice.L, L_c]
-  let w_ann := adv.annotate w
-  have h_len : w_ann.length = w.length := by
-    simp [w_ann, Advice.annotate, zip_words, adv.len]
-
-  change ((AdvCALc c).comp w_ann ((AdvCALc c).t w_ann.length) 0) ↔ (adv.f w).getLast? = some c
-  dsimp [AdvCALc]
-  rw [DiagonalShiftCA_comp_p0]
-
-  cases h_w : w.length with
-  | zero =>
-    have h_nil : w = [] := List.length_eq_zero_iff.mp h_w
-    subst h_nil
-    have h_ann_nil : w_ann = [] := by simp [w_ann, Advice.annotate, zip_words]
-    rw [h_ann_nil]
-    simp
-  | succ n =>
-    have h_ann_len_pos : w_ann.length > 0 := by rw [h_len, h_w]; simp
-    have h_idx : w_ann.length - 1 < w_ann.length := by omega
-
-    rw [List.getElem?_eq_getElem (h:=h_idx)]
-    simp
-
-    have h_idx_f : (adv.f w).length - 1 < (adv.f w).length := by
-      rw [adv.len]
-      rw [h_len] at h_idx
-      exact h_idx
-
-    have h_snd : (w_ann[w_ann.length - 1]).2 = (adv.f w)[(adv.f w).length - 1] := by
-      simp [w_ann, Advice.annotate, zip_words]
-
-    rw [h_snd]
-
-    have h_f_ne : adv.f w ≠ [] := by
-      rw [← List.length_pos_iff_ne_nil]
-      rw [adv.len, h_w]
-      simp
-
-    rw [List.getLast?_eq_some_getLast h_f_ne]
-    rw [List.getLast_eq_getElem]
-    simp
+  rw [tCellAutomatonWithAdvice.elem_L_iff]
+  rw [L_c]
+  rw [prop_of_elem_prop_set]
 
 
-end LcInRt
+  by_cases h: w = []
+  · simp [h, CA_adv_L_c]
+
+  unfold CA_adv_L_c
+  rw [fix_empty_spec]
+  simp [h]
+
+  rw [←trace_rt_L (by simp_all)]
+
+  convert_to (((List.getLast ((adv.annotate w).map Prod.snd) (by simp_all))) = c ↔ List.getLast? (adv.f w) = some c)
+  · simp
+
+  unfold Advice.annotate
+  simp only [←Word.snd.eq_1]
+  simp
+  grind
+
+
 
 lemma L_c_in_rt (adv: Advice α Γ) (h: adv.rt_closed) (c: Γ) :
-      ∃ M : tCellAutomaton α, M ∈ CA_rt α ∧ M.L = L_c adv c := by
-  let O := LcInRt.O adv c
-  have h_in : O.L ∈ ℒ (CA_rt (α × Γ) + adv) := by
-    use O
-    constructor
-    · change O ∈ tCellAutomatonWithAdvice.with_advice (CA_rt (α × Γ)) adv
-      simp [tCellAutomatonWithAdvice.with_advice]
-      use LcInRt.AdvCALc c
-      exact ⟨LcInRt.myCA_in_rt c, rfl⟩
-    · rfl
+    ∃ C : CA_rt α, C.val.L = L_c adv c := by
+  have := tCellAutomatonWithAdvice.exists_CA_rt_of_rt_closed h (CA_adv_L_c α c)
+  rw [CA_adv_L_c_spec] at this
+  exact this
 
-  erw [h] at h_in
-  rcases h_in with ⟨M, hM_in, hM_L⟩
-  use M
-  constructor
-  · exact hM_in
-  · change DefinesLanguage.L M = L_c adv c
-    rw [← hM_L, LcInRt.O_L_eq_L_c]
 
-noncomputable def CALc (adv: Advice α Γ) (h: adv.rt_closed) (c: Γ) : tCellAutomaton α :=
+noncomputable def CA_L_c (adv: Advice α Γ) (h: adv.rt_closed) (c: Γ) : CA_rt α :=
   Classical.choose (L_c_in_rt adv h c)
 
-lemma CALc_spec_1 (adv: Advice α Γ) (h: adv.rt_closed) (c: Γ) :
-    (CALc adv h c) ∈ CA_rt α :=
-  (Classical.choose_spec (L_c_in_rt adv h c)).1
-
-lemma CALc_spec_2 (adv: Advice α Γ) (h: adv.rt_closed) (c: Γ) :
-    (CALc adv h c).L = L_c adv c :=
-  (Classical.choose_spec (L_c_in_rt adv h c)).2
+@[simp]
+lemma CA_L_c_spec (adv: Advice α Γ) (h: adv.rt_closed) (c: Γ) :
+    (CA_L_c adv h c).val.L = L_c adv c :=
+  Classical.choose_spec (L_c_in_rt adv h c)
 
 
 
@@ -158,14 +88,21 @@ namespace PrefixStableProof
 
   variable (adv: Advice α Γ) (h1: adv.rt_closed)
 
-  noncomputable abbrev M_prod := ProdCA (fun c => (CALc adv h1 c).toCellAutomaton)
 
   noncomputable def first_true_or_default (q: Γ → Bool) : Γ :=
     let valid_c := Finset.univ.filter (fun c => q c)
     valid_c.toList.head?.getD default
 
+  lemma first_true_or_default_spec (x: Γ): first_true_or_default (fun c => decide (x = c)) = x := by
+    unfold first_true_or_default
+    have : (Finset.univ.filter (fun c => decide (x = c))) = {x} := by
+      ext
+      simp [eq_comm]
+    rw [this]
+    simp
+
   noncomputable def ts_adv : TwoStageAdvice α Γ := {
-    C := (M_prod adv h1).map_project first_true_or_default
+    C := (ProdCA (fun c => (CA_L_c adv h1 c).val.toCellAutomaton)).map_project first_true_or_default
     β := Γ
     M := FiniteStateTransducer.M_id Γ
   }
@@ -174,52 +111,30 @@ namespace PrefixStableProof
     grind
 
   lemma f (h2: adv.prefix_stable): (ts_adv adv h1).advice = adv := by
-    apply Advice.ext
+    apply advice_eq_iff
     funext w
-    simp [TwoStageAdvice.advice]
-    unfold ts_adv
-    simp
+    apply List.ext_getElem
+    · simp
+    intro i h_i1 h_i2
 
-    rw [ProdCA.trace_rt]
+    have w_len: i < w.length := by simp_all
 
-    apply List.ext_getElem?
+    calc ((ts_adv adv h1).advice.f w)[i]
+      _ = (first_true_or_default fun b => decide (List.take (i + 1) w ∈ L_c adv b)) := by
+        simp [TwoStageAdvice.advice, ts_adv, w_len, trace_rt_getElem_i_iff2]
 
+      _ = (first_true_or_default fun b => (adv.f w)[i] = b) := by
+        congr
+        ext b
+        congr
+        unfold L_c
+        rw [prop_of_elem_prop_set]
+        unfold Advice.prefix_stable at h2
+        rw [h2]
+        simp [List.getLast?_take, w_len]
 
-
-    intro i
-    rw [List.getElem?_map]
-    erw [ProdCA.zipMany_get?]
-    simp
-
-    by_cases h_i : i < w.length
-    case neg => simp [h_i]
-
-    unfold first_true_or_default
-    simp
-
-
-    simp [scan_temporal_in_F_pos (CALc_spec_1 adv h1 _), h_i]
-    simp [CALc_spec_2 adv h1]
-    unfold L_c
-
-    have h2 := h2 w (i+1)
-
-    -- TODO@lean: This is annoying
-    suffices
-      some ((Finset.univ.filter (fun c => List.getLast? (adv.f (List.take (i + 1) w)) = some c)).toList.head?.getD default) = (adv.f w)[i]? by
-        grind
-
-    rw [h2]
-    have : i < (adv.f w).length := by
-      simp [h_i, adv.len]
-
-    rw [getLastOfTake this]
-
-    rw [List.getElem?_eq_getElem this]
-    simp
-    have h_singleton : (Finset.univ.filter (fun c => (adv.f w)[i] = c)) = {(adv.f w)[i]} := by grind
-    rw [h_singleton]
-    simp
+      _ = (adv.f w)[i] := by
+        rw [first_true_or_default_spec]
 
 
 end PrefixStableProof
